feat new --mark-sorry flag

ImportGraphTest/Used.lean
@@ -1,1 +1,3 @@
 import ImportGraphTest.Unused
+
+def something := 2
