ImportGraph/Lean/Environment.lean
@@ -1,0 +1,22 @@
+/-
+Copyright (c) 2023 Kim Morrison. All rights reserved.
+Released under Apache 2.0 license as described in the file LICENSE.
+Authors: Kim Morrison
+-/
+module
+
+public import Lean.Environment
+
+namespace Lean
+
+/-- Return the name of the module in which a declaration was defined. -/
+public def Environment.getModuleFor? (env : Environment) (declName : Name) : Option Name :=
+  match env.getModuleIdxFor? declName with
+  | none =>
+    if env.constants.map₂.contains declName then
+      env.header.mainModule
+    else
+      none
+  | some idx => env.header.moduleNames[idx.toNat]!
+
+end Lean
