ImportGraphTest/ToTarget.lean
@@ -1,0 +1,6 @@
+import ImportGraphTest.Used
+import ImportGraphTest.WithSorry.Def
+import ImportGraphTest.WithSorry.Thm
+
+#guard_msgs in
+theorem fancy : something = 2 := rfl
